wip: linear bcc & linear rs

LinearProof.v
@@ -13,6 +13,7 @@ From Stdlib Require Import Lia.
 From Stdlib Require Import List. Import ListNotations.
 Require Import ExtLib.Data.Monads.OptionMonad.
 From SECF Require Import Maps MapsFunctor.
+
 Set Default Goal Selector "!".
 (* TERSE: /HIDEFROMHTML *)
 
@@ -169,8 +170,14 @@ Inductive multi_spec_inst (p:prog) :
   where "p |- <(( sc ))> -->m*_ ds ^^ os ^^ n <(( sct ))>" :=
     (multi_spec_inst p sc sct ds os n).
 
+From SECF Require Import sflib.
+
 Definition match_reg (p: MiniCET.prog) (r: MCC.reg) (r': reg) : Prop :=
   forall x, val_inject p (r ! x) (r' ! x).
+
+Definition match_reg_src (p: MiniCET.prog) (r: MCC.reg) (r': reg) (ms: bool) : Prop :=
+  (forall x, x <> msf /\ x <> callee -> val_inject p (r ! x) (r' ! x))
+/\ r' ! msf = N (if ms then 1 else 0).
 
 Definition match_mem (p: MiniCET.prog) (m m': mem) : Prop :=
   forall i, match nth_error m i, nth_error m' i with
@@ -213,6 +220,65 @@ Definition match_ob (p: MiniCET.prog) (o: MiniCET.observation) (o': observation)
 Definition match_obs (p: MiniCET.prog) (ds: MiniCET.obs) (ds': obs) : Prop :=
   Forall2 (match_ob p) ds ds'.
 
+(* wf *)
+
+Definition wf_dir (p: prog) (d: direction) : Prop :=
+  match d with
+  | DCall pc' => is_some (nth_error p pc') = true
+  | _ => True
+  end.
+
+Definition wf_ds (p: prog) (ds: dirs) : Prop :=
+  Forall (wf_dir p) ds.
+
+Lemma pc_inj_iff p pc l :
+  pc_inj p pc = Some l <-> pc_inj_inv p l = Some pc.
+Proof.
+  unfold pc_inj, pc_inj_inv. destruct pc. split.
+  - eapply coord_flat_inverse.
+  - eapply flat_coord_inverse.
+Qed.
+
+Lemma src_inv
+  (p: MiniCET.prog) (tp: prog) pc l i
+  (TRANSL: machine_prog p = Some tp)
+  (SRC: p[[pc]] = Some i)
+  (INJ: pc_inj p pc = Some l) :
+  nth_error tp l = Some i.
+Proof.
+Admitted.
+
+Lemma tgt_inv
+  (p: MiniCET.prog) (tp: prog) pc l i
+  (TRANSL: machine_prog p = Some tp)
+  (TGT: nth_error tp l = Some i)
+  (INJ: pc_inj p pc = Some l) :
+  p[[pc]] = Some i.
+Proof.
+Admitted.
+
+Lemma wf_dir_inj
+  (p: MiniCET.prog) (tp: prog) d td
+  (TRANSL: machine_prog p = Some tp)
+  (WFT: wf_dir tp td)
+  (MATCH: match_dir p d td):
+  wf_dir' p d.
+Proof.
+  destruct td; ss; des_ifs_safe.
+  { red in MATCH. des_ifs. }
+  red in MATCH. des_ifs.
+  admit.
+Admitted.
+
+Lemma wf_ds_inj
+  (p: MiniCET.prog) (tp: prog) ds tds
+  (TRANSL: machine_prog p = Some tp)
+  (WFT: wf_ds tp tds)
+  (MATCH: match_dirs p ds tds):
+  wf_ds' p ds.
+Proof.
+Admitted.
+
 Lemma minicet_linear_bcc_single
   (p: MiniCET.prog) (tp: prog) sc tc tct tds tos
   (TRANSL: machine_prog p = Some tp)
@@ -235,4 +301,90 @@ Lemma minicet_linear_bcc
              /\ match_states p sct tct
              /\ match_dirs p ds tds /\ match_obs p os tos.
 Proof.
+Admitted.
+
+Definition spec_same_obs_machine p pc r1 r2 m1 m2 stk b : Prop :=
+  forall ds n os1 os2 c1 c2 (WFDS: wf_ds p ds),
+  p |- <(( S_Running (pc, r1, m1, stk, b, false) ))> -->m*_ds^^os1^^n <(( c1 ))> ->
+  p |- <(( S_Running (pc, r2, m2, stk, b, false) ))> -->m*_ds^^ os2^^n <(( c2 ))> ->
+  (Utils.prefix os1 os2) \/ (Utils.prefix os2 os1).
+
+Definition relative_secure_machine (p:MiniCET.prog) (tp: prog) (trans : MiniCET.prog -> option prog)
+  (r1 r2 r1' r2' : reg) (m1 m2 m1' m2' : mem) : Prop :=
+  seq_same_obs p (0,0) r1 r2 m1 m2 [] ->
+  match_reg_src p r1 r1' false -> match_reg_src (uslh_prog p) r2 r2' false ->
+  match_mem p m1 m1' -> match_mem p m2 m2' ->
+  trans p = Some tp ->
+  spec_same_obs_machine tp 0 r1' r2' m1' m2' [] true.
+
+Lemma spec_eval_relative_secure_machine
+  p r1 r2 r1' r2' m1 m2 m1' m2' tp
+  (FST: first_blk_call p)
+  (NCT: no_ct_prog p)
+  (WFP: wf_prog p)
+  (NEM1: nonempty_mem m1)
+  (NEM2: nonempty_mem m2)
+  (CALLEE1: r1' ! callee = N 0)
+  (CALLEE2: r2' ! callee = N 0)
+  (SAFE1: seq_exec_safe p ((0,0), r1, m1, []))
+  (SAFE2: seq_exec_safe p ((0,0), r2, m2, []))
+  (UNUSED1: unused_prog msf p)
+  (UNUSED2: unused_prog callee p) :
+  relative_secure_machine p tp (fun p => machine_prog (uslh_prog p)) r1 r2 r1' r2' m1 m2 m1' m2'.
+Proof.
+  red. i.
+  set (ir1 := (msf !-> N 0; callee !-> (FP 0); r1)).
+  set (ir2 := (msf !-> N 0; callee !-> (FP 0); r2)).
+
+  hexploit (spec_eval_relative_secure p r1 r2 ir1 ir2 m1 m2); eauto.
+  intros REL. red in REL.
+
+  assert (IREG1: Rsync r1 ir1 false).
+  { split; subst ir1; ss. ii. des.
+    do 2 (rewrite MiniCET_Index.t_update_neq; eauto). }
+
+  assert (IREG2: Rsync r2 ir2 false).
+  { split; subst ir2; ss. ii. des.
+    do 2 (rewrite MiniCET_Index.t_update_neq; eauto). }
+
+  hexploit REL; eauto.
+  intros SPEC.
+
+  hexploit seq_spec_safety_preservation_init; try eapply SAFE1; eauto.
+  { subst ir1. rewrite MiniCET_Index.t_update_neq; eauto. ii; clarify. }
+  intros ISAFE1.
+
+  hexploit seq_spec_safety_preservation_init; try eapply SAFE2; eauto.
+  { subst ir2. rewrite MiniCET_Index.t_update_neq; eauto. ii; clarify. }
+  intros ISAFE2.
+
+  red. i.
+  hexploit minicet_linear_bcc; [|eapply ISAFE1| |eapply H5|]; eauto.
+  { econs; ss.
+    - unfold pc_inj. admit. (* nonempty *)
+    - red. i. red in H0.
+      destruct (string_dec x callee).
+      { subst. subst ir1. rewrite CALLEE1. ss.
+        admit. }
+      destruct (string_dec x msf).
+      { des. subst. subst ir1. rewrite H7. ss. }
+      des. exploit H0; eauto. i. des. eauto.
+      inv IREG1. rewrite <- H8; eauto.
+      unfold val_inject in *. des_ifs_safe.
+      admit.
+    - red. i. specialize (H2 i). des_ifs_safe.
+      unfold val_inject in *. des_ifs_safe. admit. }
+  i. des.
+  hexploit minicet_linear_bcc; [|eapply ISAFE2| |eapply H6|]; eauto.
+  { admit. (* see above *) }
+  i. des.
+
+  assert (UNIQ: ds0 = ds1).
+  { admit. }
+  subst.
+  red in SPEC. hexploit SPEC; cycle 1.
+  { eapply H7. }
+  { eapply H11. }
+  2:{ eapply wf_ds_inj; eauto. }
+  i. admit. (* H15 H14 H10 *)
 Admitted.
